Temporal_Planning_Base/Sequences.thy
@@ -912,7 +912,20 @@ begin
       apply (rule ext_seq_induct_list_prop_and_post[where P = P and Q = Q and R = R])
       using assms base step by auto
   qed
-  
+
+  lemma ext_seq_comp_seq_apply_induct_list_prop_composable':
+    assumes LPxsRxn: "LP xs \<and> R (last xs)"
+        and PQ: "\<And>i s. i < length fs \<Longrightarrow> P i s \<Longrightarrow> Q i ((fs ! i) s)"
+        and ind: "\<And>i s. i < length fs \<Longrightarrow> P i s \<Longrightarrow> Q i ((fs ! i) s) \<Longrightarrow> LP [s, (fs ! i) s]"
+        and QP: "\<And>i s. Suc i < length fs \<Longrightarrow> Q i s \<Longrightarrow> P (Suc i) s"
+        and RPn: "\<And>x. 0 < length fs \<Longrightarrow> R x \<Longrightarrow> P 0 x"
+        and QSl: "\<And>x. 0 < length fs \<Longrightarrow> Q (length fs - 1) x \<Longrightarrow> S x"
+        and RSn: "\<And>x. length fs = 0 \<Longrightarrow> R x \<Longrightarrow> S x"
+        and SR1: "\<And>x. S x \<Longrightarrow> R' x"
+      shows "LP ((ext_seq o seq_apply) fs xs) \<and> R' (last ((ext_seq o seq_apply) fs xs))"
+    apply (rule ext_seq_comp_seq_apply_induct_list_prop_composable[where P = P and Q = Q and R = R])
+    using assms by auto (* context_conjI *)
+
   lemma ext_seq_comp_seq_apply_single_list_prop_and_post:
     assumes LPxsRxn: "LP xs \<and> R (last xs)"
         and ind_step: "\<And>x. R x \<Longrightarrow> S (f x) \<and> LP [x, f x]"
